HexGraphIso/Nauty/Correct/Exit/Final.lean
@@ -96,7 +96,7 @@ theorem ofCheap {G : Colored n k} {ctx : Ctx n}
       (initialPartition G).1 1
       (fmptn r.lab r.ptn level n).1
       (fmptn r.lab r.ptn level n).2 := by
-    apply pairOk_fmptn_of_subtree (ctx := ctx) (G := G)
+    apply SubtreeOk.pair_ok (ctx := ctx) (G := G)
       (r := r) hinv.nonempty hinv.positive
     · rw [hg]
       exact size_rowsOf G
